osiris/src/Syntax.ml
@@ -392,4 +392,6 @@ and sitem =
   (* An [include] directive [include me]. *)
   | IInclude of mexpr
 
+  | IExternal of var * expr
+
   | IExtend of name list
