rocq-osiris/theories/proofmode/pure_tactics.v
@@ -876,6 +876,7 @@ Ltac2 rec unfold_item (item : constr) : constr :=
          | IModule _ _ => Control.zero Match_failure
          | IOpen ?i => get_ref i
          | IInclude ?me => get_ref me
+         | IExternal _ ?a => get_ref a
          | IExtend ?ns => get_ref ns
          end
        in
@@ -906,6 +907,11 @@ Ltac2 init_item (item : constr) (spec : constr option) () :=
       end
   | ILetRec _ => eapply struct_letrec
   | IModule _ _ => eapply struct_module
+  | IExternal _ _ =>
+      match spec with
+      | None => eapply struct_external
+      | Some spec => eapply struct_external with (spec := $spec)
+      end
   end.
 
 Ltac2 next_item0 (spec : constr option) () :=
